Reach capabilities and the subcapturing rule

CC/CaptureSet.lean
@@ -6,22 +6,24 @@ namespace CC
 
 structure CaptureSet (n : Nat) where
   elems : Finset (Fin n)
+  reachElems: Finset (Fin n)
+  hasCap : Bool
 
 instance : Membership (Fin n) (CaptureSet n) :=
   ⟨fun a s => a ∈ s.1⟩
 
 instance : Singleton (Fin n) (CaptureSet n) :=
-  ⟨fun x => ⟨{x}⟩⟩ 
+  ⟨fun x => ⟨{x}, ∅, false⟩⟩
 
 instance : Union (CaptureSet n) :=
-  ⟨fun s t => ⟨s.1 ∪ t.1⟩⟩ 
+  ⟨fun s t => ⟨s.1 ∪ t.1, s.2 ∪ t.2, s.3 ∨ t.3⟩⟩
 
 instance : EmptyCollection (CaptureSet n) :=
-  ⟨⟨{}⟩⟩
+  ⟨⟨{}, {}, false⟩⟩
 
 def CaptureSet.rename (C : CaptureSet n1) (f : VarMap n1 n2) : CaptureSet n2 :=
-  ⟨C.elems.image f⟩
-  
+  ⟨C.elems.image f, C.reachElems.image f, C.hasCap⟩
+
 def CaptureSet.weaken_var (C : CaptureSet n) : CaptureSet n.succ :=
   C.rename weaken_map
 
@@ -33,6 +35,11 @@ theorem rename_singleton (x : Fin n) (f : VarMap n n') :
   CaptureSet.rename {x} f = {f x} := by
   simp [CaptureSet.rename]
   aesop
+
+@[simp]
+theorem rename_singleton_reach (x : Fin n) (f : VarMap n n') :
+  CaptureSet.rename ⟨∅, {x}, false⟩ f = ⟨∅, {f x}, false⟩ := by
+  simp [CaptureSet.rename]
 
 @[simp]
 theorem rename_empty (f : VarMap n n') :
@@ -56,7 +63,9 @@ theorem mem_rename {C : CaptureSet n} :
   simp only [CaptureSet.rename, mem_def]
   aesop
 
-theorem union_def {C1 C2 : CaptureSet n} : C1 ∪ C2 = ⟨C1.1 ∪ C2.1⟩ := rfl
+theorem union_def {C1 C2 : CaptureSet n} :
+  C1 ∪ C2 = ⟨C1.1 ∪ C2.1, C1.2 ∪ C2.2, C1.3 ∨ C2.3⟩ :=
+  rfl
 
 @[simp]
 theorem CaptureSet.rename_id : ∀ {C : CaptureSet n},
@@ -82,12 +91,15 @@ theorem CaptureSet.rename_union {C1 C2 : CaptureSet n} :
 def CaptureSet.open_var (C : CaptureSet n.succ) (z : Fin n) : CaptureSet n :=
   C.rename (open_map z)
 
-lemma CaptureSet.val_eq {C1 C2 : CaptureSet n} (h : C1.elems = C2.elems) :
-  C1 = C2 := 
+lemma CaptureSet.val_eq {C1 C2 : CaptureSet n}
+  (h1 : C1.elems = C2.elems)
+  (h2 : C1.reachElems = C2.reachElems)
+  (h3 : C1.hasCap = C2.hasCap) :
+  C1 = C2 :=
   by cases C1; cases C2; aesop
 
 lemma CaptureSet.val_def :
-  ({ elems := xs } : CaptureSet n).elems = xs := rfl
+  ({ elems := xs, reachElems := ys, hasCap := u } : CaptureSet n).elems = xs := rfl
 
 lemma CaptureSet.in_union_elems {C1 C2 : CaptureSet n}
   (h : x ∈ (C1 ∪ C2).elems) :
@@ -98,4 +110,3 @@ lemma CaptureSet.in_union_elems {C1 C2 : CaptureSet n}
 
 def CaptureSet.weaken_var1 (C : CaptureSet (Nat.succ n)) : CaptureSet n.succ.succ :=
   C.rename weaken_map.ext
-  
