CC/Subcapt/Subst.lean
@@ -38,3 +38,4 @@ def Subcapt.subst (σ : VarSubst Γ Δ f) :
     rw [rename_singleton] at h
     rw [<- eq2]
     assumption
+  case sc_reach => simp; apply Subcapt.sc_reach
